Add for loop to Go semantics
The Go.For loop takes a variable, termination expression, and body, and
executes the body as long as the variable is less than the termination
expression. After each execution of the body, the variable is
incremented by one. This corresponds to a very limited for loop - it is
over one variable, does not initialize the variable, and increments
exactly by one every time. The reasoning here is that the body and
termination condition are fairly general, so without restricting the
body to progs that don't modify the variable, it's not reasonable to
bind the variable to a value for each iteration of the loop, which was
another possible incarnation.

With this patch, the Go.For loop  exists and is well-defined, but there
is no extraction code to produce it yet.

src/Go.v
@@ -137,6 +137,7 @@ Module Go.
   | Seq : stmt -> stmt -> stmt
   | If : expr -> stmt -> stmt -> stmt
   | While : expr -> stmt -> stmt
+  | For : var -> expr -> stmt -> stmt
   | Call (retvars: list var) (* The caller's variables to get the return values *)
          (f: label) (* The function to call *)
          (argvars: list var) (* The caller's variables to pass in *)
@@ -170,6 +171,10 @@ Module Go.
       forall cond body,
         source_stmt body ->
         source_stmt (While cond body)
+  | SFor :
+      forall v term body,
+      source_stmt body ->
+      source_stmt (For v term body)
   | SCall : forall retvars f argvars, source_stmt (Call retvars f argvars)
   | SAssign : forall x e, source_stmt (Assign x e)
   | SDeclare :
@@ -394,6 +399,7 @@ Module Go.
         | Some kk => VarMap.add kk v m
       end.
 
+    Definition increment v := Assign v (Binop Plus (Var v) (Const Num 1)).
 
     Inductive runsto : stmt -> state -> state -> Prop :=
     | RunsToSkip : forall st,
@@ -420,6 +426,16 @@ Module Go.
                            let loop := While cond body in
                            is_false (snd st) cond ->
                            runsto loop st st
+    | RunsToForTrue : forall v term body st st' st'',
+                            let loop := For v term body in
+                            is_true (snd st) (TestE Lt (Var v) term) ->
+                            runsto body st st' ->
+                            runsto (Seq (increment v) loop) st' st'' ->
+                            runsto loop st st''
+    | RunsToForFalse : forall term v body st,
+                            let loop := For v term body in
+                            is_false (snd st) (TestE Lt (Var v) term) ->
+                            runsto loop st st
     | RunsToDeclare : forall body body' d s si si' s' d' var t,
                        VarMap.find var s = None ->
                        si = VarMap.add var (default_value t) s ->
@@ -480,6 +496,15 @@ Module Go.
                          let loop := While cond body in
                          is_false (snd st) cond ->
                          step (st, loop) (st, Skip)
+    | StepForTrue : forall v term body st,
+                      let loop := For v term body in
+                      is_true (snd st) (TestE Lt (Var v) term) ->
+                      step (st, loop) (st, Seq body
+                                          (Seq (increment v) loop))
+    | StepForFalse : forall v term body st,
+                       let loop := For v term body in
+                       is_false (snd st) (TestE Lt (Var v) term) ->
+                       step (st, loop) (st, Skip)
     | StepDeclare : forall t body body' d s s' var,
                       VarMap.find var s = None ->
                       s' = VarMap.add var (default_value t) s ->
@@ -674,6 +699,16 @@ Module Go.
                              let loop := While cond body in
                              is_false (snd st) cond ->
                              runsto_InCall loop st st
+    | RunsToICForTrue : forall v term body st st' st'',
+                            let loop := For v term body in
+                            is_true (snd st) (TestE Lt (Var v) term) ->
+                            runsto_InCall body st st' ->
+                            runsto_InCall (Seq (increment v) loop) st' st'' ->
+                            runsto_InCall loop st st''
+    | RunsToICForFalse : forall v term body st,
+                            let loop := For v term body in
+                            is_false (snd st) (TestE Lt (Var v) term) ->
+                            runsto_InCall loop st st
     | RunsToICDeclare : forall body body' d s si si' s' d' var t,
                           VarMap.find var s = None ->
                           si = VarMap.add var (default_value t) s ->
@@ -728,6 +763,13 @@ Module Go.
 
     Hint Constructors source_stmt.
 
+    Lemma source_stmt_increment : forall v, source_stmt (increment v).
+    Proof.
+      unfold increment. eauto.
+    Qed.
+
+    Hint Resolve source_stmt_increment.
+
     Lemma source_stmt_RunsToInCall_runsto :
       forall p,
         source_stmt p ->
@@ -735,7 +777,7 @@ Module Go.
           runsto_InCall p st st' ->
           runsto p st st'.
     Proof.
-      induction 2; intros; subst_definitions; invc H; eauto.
+      induction 2; intros; subst_definitions; invc H; eauto 10.
     Qed.
 
     Hint Resolve source_stmt_RunsToInCall_runsto.
@@ -769,6 +811,7 @@ Module Go.
     Proof.
       intros.
       prep_induction H0; induction H0; intros; subst_definitions; subst; do_inv.
+      - subst_definitions. eauto.
       - subst_definitions. eauto.
       - destruct st', st''. invc H0_0. eauto.
       - eapply RunsToICCallOp; eauto. assert (Some input = Some input0) by congruence. find_inversion. auto.
